ulib/tactics_ml/FStar_Tactics_Builtins.ml
@@ -156,6 +156,7 @@ let pack                    = from_tac_1 B.pack
 let curms                   = from_tac_1 B.curms
 let set_urgency             = from_tac_1 B.set_urgency
 let t_commute_applied_match = from_tac_1 B.t_commute_applied_match
+let gather_or_solve_explicit_guards_for_resolved_goals = from_tac_1 B.gather_explicit_guards_for_resolved_goals
 
 (* sigh *)
 let fix_either (s : ('a, 'b) either) : ('a, 'b) either =
