tests/bug-reports/Bug2635.fst
@@ -8,7 +8,8 @@ let prove_False
   : squash False
   = pf
 
-[@@expect_failure]
+//This fails with error 217, correctly complaining that the solved goal does not have type False
+[@@expect_failure [217]]
 let absurd : squash False
   = _ by (// |- ?pf : squash l_False
           apply (`prove_False);
@@ -16,10 +17,63 @@ let absurd : squash False
           // (pf0 : squash l_False) |- _ : ?pf == ()
           trefl ())
 
+//Using the  gather_explicit_guards_for_resolved_goals primitive
+//you can now see that goal explicitly and work on solving from your tactic
+let admit_absurd (_:unit) : squash False
+  = _ by (// |- ?pf : squash l_False
+          apply (`prove_False);
+          let pf0 = intro () in
+          // (pf0 : squash l_False) |- _ : ?pf == ()
+          trefl ();
+          gather_or_solve_explicit_guards_for_resolved_goals();
+          dump "After";
+          tadmit())
+
+
+
 // Revised version, not depending on False by Aseem
 assume
 val p : Type0
 
+assume
+val q (x:pos) : Type0
+
+//the primitive is perhaps more useful in a context like this
+assume
+val expect_pos (_: squash (exists (x:pos). q x)) : squash p
+
+let intro_exists (#a:Type)  (#p:a -> Type) (x:a) (_:squash (p x)) : squash (exists (x:a). p x) = ()
+
+[@@expect_failure [217]]
+let use_pos (x:nat) (xpos:squash (x > 0)) (hyp:squash (q x)) =
+  assert p by (
+    apply (`expect_pos);
+    apply (`intro_exists);
+    apply (quote hyp)) //the implicit `pos` of intro_exists is solved by unification here to x:nat
+
+let use_pos (x:nat) (xpos:squash (x > 0)) (hyp:squash (q x)) =
+  assert p by (
+    apply (`expect_pos);
+    apply (`intro_exists);
+    apply (quote hyp); //the implicit `pos` of intro_exists is solved by unification here to x:nat
+    //can pick up the goal explicitly to prove that x > 0
+    gather_or_solve_explicit_guards_for_resolved_goals ();
+    let _ = implies_intro () in
+    apply (quote xpos))
+
+let use_one (hyp:squash (q 1)) =
+  assert p by (
+    apply (`expect_pos);
+    apply (`intro_exists);
+    apply (quote hyp); //the implicit `pos` of intro_exists is solved by unification here to 1:nat
+    //and F* does not accept that implicitly
+    //but you can ask F* to solve it by simplification
+    gather_or_solve_explicit_guards_for_resolved_goals ())
+
+
+//////////////////////////////////////////////////////////////
+// Some other variants and test cases
+//////////////////////////////////////////////////////////////
 let test (pr:squash p) (f: (unit -> squash (pr == ()))) : squash p = pr
 
 [@@expect_failure]
